type 'mkobj' in the paper
COMPARING OBJECT ENCODINGS

theories/typing/examples/records.v
@@ -6,22 +6,6 @@ From lrust.typing Require Export type.
 From lrust.typing Require Import typing.
 From iris.prelude Require Import options.
 
-Check (Closed [] (rec: "mkobj" ["repr"] :=
-  "repr" ↓ "x")%V).
-Compute (Closed [] (rec: "mkobj" ["repr"] :=
-  "repr" ↓ "x")%V).
-
-Check (Closed ("mkobj" :b: ["repr"]%binder +b+ []) ("repr" ↓ "x")%E).
-Compute (Closed ("mkobj" :b: ["repr"]%binder +b+ []) ("repr" ↓ "x")%E).
-
-Definition obj_test : val :=
-  rec: "mkobj" ["repr"] :=
-    "repr" ↓ "x".
-
-    (* "get" r: "repr" ↓ "x" :r: 
-    "set" r: (λ: ["n"], ("mkobj" ["x" r: "n" :r: rnil])) :r:
-    "bump" r: ("mkobj" [ ("x" r: (("repr" ↓ "x") + #1) :r: rnil)%E ]) :r: rnil%E. *)
-
 Section record.
 Context `{!typeGS Σ}.
 Notation iProp := (iProp Σ).
@@ -56,23 +40,19 @@ Proof.
   iSplit; first done. iSplit; first done. rewrite /rnil' //.
 Qed.
 
-Definition try_obj : val := rec: "mkobj" ["repr"] :=
-  "get" r: "repr" ↓ "x" :r: 
-  "set" r: (λ "n", "mkobj" ["x" r: "n" :r: rnil]) :r:
-  "bump" : "mkobj" ["x" : "repr" ↓ "x" + #1] :r: rnil
-
-Definition obj_pre t := record [("x", int); ("y", int); ("area", box t)].
+(* `{!TyWf t} *)
+Definition fn_ty t := fn (λ _: (), FP (λ ϝ, ∅ ϝ) Vector.nil t).
+Definition obj_pre t : type := record [("x", int); ("y", int); ("area", fn_ty t)].
 Definition obj_pre1 t := record [("x", int); ("y", int); ("area", box t)].
 
 Local Instance obj_contractive : TypeContractive obj_pre.
 Proof.
   intros n o1 o2 Ho.
   rewrite /obj_pre.
-  replace ([("x", int); ("y", int); ("area", box o1)]) with (zip ["x"; "y"; "area"] [int; int; box o1]); last done.
-  replace ([("x", int); ("y", int); ("area", box o2)]) with (zip ["x"; "y"; "area"] [int; int; box o2]); last done.
+  replace ([("x", int); ("y", int); ("area", fn_ty o1)]) with (zip ["x"; "y"; "area"] [int; int; fn_ty o1]); last done.
+  replace ([("x", int); ("y", int); ("area", fn_ty o2)]) with (zip ["x"; "y"; "area"] [int; int; fn_ty o2]); last done.
   apply record_proper. (* well I guess f_equiv can't detect this directly*)
-  repeat f_equiv.
-  apply Ho.
+  rewrite /fn_ty. repeat f_equiv; simpl; [done | apply Ho].
 Qed.
 
 Local Instance obj_contractive1 : TypeContractive obj_pre1.
@@ -94,5 +74,126 @@ Proof.
   apply fixpoint_mono. intros. unfold obj_pre, obj_pre1.
   admit.
 Admitted.
-(* TODO *)
+
+Definition set_fn t := fn (λ _: (), FP (λ ϝ, ∅ ϝ) (Vector.cons int Vector.nil) t).
+Definition counter_pre t : type := record [("get", int); ("set",  set_fn t); ("bump", box t)].
+
+Local Instance counter_contractive : TypeContractive counter_pre.
+Proof.
+  intros n t1 t2 Ht.
+  rewrite /counter_pre.
+  replace ([("get", int); ("set", set_fn t1); ("bump", box t1)])
+    with (zip ["get"; "set"; "bump"] [int; set_fn t1; box t1]); last done.
+  replace ([("get", int); ("set", set_fn t2); ("bump", box t2)])
+    with (zip ["get"; "set"; "bump"] [int; set_fn t2; box t2]); last done.
+  apply record_proper. rewrite /set_fn.
+  repeat f_equiv; simpl; first f_equiv; apply Ht.
+Qed.
+
+Definition mkobj_fn : val := fnrec: "mkobj" ["repr'"] :=
+  let: "repr" := !"repr'" in
+  let: "proj" := "repr" ↓ "x" in
+  let: "set_fn" := (fn: ["n"] :=
+    let: "n'" := !"n" in
+    let: "rec" := "x" r: "n'" :r: rnil in
+    let: "pp" := new [(#2)%V] in
+    "pp" <- "rec";;         (* don't know why it has to add a % *)
+    letcall: "obj" := "mkobj" ["pp"]%E in
+    "return" ["obj"]) in
+  let: "proj1" := "proj" + "proj" in
+  let: "rec" := "x" r: "proj1" :r: rnil in
+  let: "pp" := new [(#2)%V] in
+  "pp" <- "rec";;
+  letcall: "bumped" := "mkobj" ["pp"]%E in
+  let: "last" := "bump" r: "bumped" :r: rnil in
+  let: "middle" := "set" r: "set_fn" :r: "last" in
+  let: "r" := "get" r: "proj" :r: "middle" in
+  let: "rp" := new [(#4)%V] in
+  "rp" <- "r";;
+  "return" ["rp"].
+
+Definition repr_ty := record [("x", int)].
+Definition counter_ty := type_fixpoint counter_pre.
+
+Local Lemma counter_unfold :
+  counter_ty ≡ counter_pre counter_ty.
+Proof. apply type_fixpoint_unfold. Qed.
+
+Lemma counter_size : counter_ty.(ty_size) = 4%nat.
+Proof. rewrite counter_unfold //. Qed.
+
+Lemma counter_typed `{!TyWf repr_ty} `{!TyWf counter_ty} : typed_val mkobj_fn (fn(∅; repr_ty) → counter_ty).
+Proof.
+  intros E L. rewrite /mkobj_fn /repr_ty.
+  iApply type_rec; [done |].
+  iIntros "/= !>".
+  iIntros (?????).
+  inv_vec args=>?. simpl_subst.
+  iApply type_deref'; [solve_typing..| ].
+  iIntros (r). simpl_subst.
+  iApply (type_proj _ _ _ _ _ _ int _ _ _ [("x", int)]); [done | solve_typing.. |].
+  iIntros (v). simpl_subst.
+  (*               E L T T' T1 *)
+  iApply (type_let _ _ _ _ [f ◁ (fn(∅; repr_ty) → counter_ty)]); [ | solve_typing |].
+  {
+    iApply (type_fn _ _ _ _ _ 1%nat
+    (* the setter type *)
+    (λ _: (), FP (λ ϝ, ∅ ϝ) (Vector.cons int Vector.nil) counter_ty)); 
+      [solve_typing..|].
+  iIntros "!>" (????).
+  inv_vec args=>?. simpl_subst.
+  iApply type_deref; [solve_typing..|].
+  iIntros (?). simpl_subst.
+  (* tctx_extract_ctx T1 T2 T3: means we can
+    split T2 into T1 and T3 (and the rest),
+    it's not the other direction... *)
+  iApply type_rcons'; [solve_typing|].
+  iIntros (?). simpl_subst.
+  iApply type_new; [solve_typing..|].
+  iIntros (p); simpl_subst.
+  iApply type_assign; [solve_typing..|].
+    (*                   x E L C T T'*)
+    iApply (type_letcall _ _ _ _ _ _).
+    - rewrite Forall_singleton. solve_closed.
+    - solve_typing.
+    - solve_typing.
+    - intros. simpl. admit.
+    - simpl. solve_typing.
+    - iIntros (?). simpl_subst. iApply type_jump; solve_typing.
+  }
+  iIntros (setter). simpl_subst.
+  iApply type_plus; [solve_typing|].
+  iIntros (?); simpl_subst.
+  iApply type_rcons'; [solve_typing|].
+  iIntros (?); simpl_subst.
+  iApply type_new; [solve_typing..|].
+  iIntros (p); simpl_subst.
+  iApply type_assign; [solve_typing..|].
+  iApply type_letcall; [solve_typing..|].
+  iIntros (?); simpl_subst.
+  iApply type_rcons'; [solve_typing..|].
+  iIntros (?); simpl_subst.
+  iApply type_rcons; [solve_typing|].
+  iIntros (?); simpl_subst.
+  iApply type_rcons; [solve_typing|].
+  iIntros (?); simpl_subst.
+  iApply type_new; [solve_typing..|].
+  iIntros (?); simpl_subst.
+  replace (fn (λ _ : (),
+    {|
+      fp_E := λ ϝ0 : lft, ∅ ϝ0;
+      fp_tys := [#int];
+      fp_ty := counter_ty
+    |})) with (set_fn counter_ty); last done.
+  iApply (type_assign _ _ (box counter_ty)); [solve_typing | | ].
+  - replace (rcons ("get", int)
+      (rcons ("set", set_fn counter_ty)
+      (rcons ("bump", box counter_ty) rnil'))) 
+      with (counter_pre counter_ty); last done.
+    replace (counter_pre counter_ty) with counter_ty.
+    + rewrite /box counter_size. iApply write_own. rewrite counter_size //.
+    + clear. admit. (* rewrite counter_unfold. apply leibniz_equiv. *)
+  - iApply type_jump; [solve_typing.. ].
+  Admitted.
+
 End typing.
