theories/typing/record.v
@@ -114,13 +114,44 @@ Section record.
     do 2 rewrite H1.
     apply rcons_proper; first apply H. apply IHForall2.
   Qed.
+  Global Instance record_wf fl tyl `{!ListTyWf tyl} : TyWf (record (zip fl tyl)) :=
+    { ty_lfts := tyl_lfts tyl; ty_wf_E := tyl_wf_E tyl }.
 
 End record.
 
 Section typing.
 Context `{!typeGS Σ}.
+  Lemma tctx_incl_rnil_singleton E L T : tctx_incl E L T [rnil%V ◁ rnil'].
+  Proof.
+    iIntros (???) "_ _ $ _ !>".
+    rewrite tctx_interp_singleton /tctx_elt_interp.
+    iExists rnil%V; iSplit; done.
+  Qed.
 
-  Lemma type_rcons E L l p1 p2 t1 t2: 
+  Lemma tctx_extract_ctx_rnil E L T1 T2 T3 :
+    tctx_extract_ctx E L T1 T2 T3 → tctx_extract_ctx E L ((rnil%V ◁ rnil') :: T1) T2 T3.
+  Proof.
+    rewrite /tctx_extract_hasty.
+    apply tctx_extract_ctx_hasty,
+      (tctx_incl_frame_r T2 [] [rnil%V ◁ rnil']),
+      tctx_incl_rnil_singleton.
+  Qed.
+
+  Lemma tctx_incl_rnil E L T1 T2 :
+    tctx_incl E L T1 T2 → tctx_incl E L T1 ((rnil%V ◁ rnil') :: T2).
+  Proof.
+    iIntros (Hincl ???) "Hlft HEl q T".
+    iMod (Hincl with "Hlft HEl q T") as "[q HT]".
+    rewrite tctx_interp_cons tctx_hasty_val.
+    iModIntro. iFrame. done.
+  Qed.
+
+  Fixpoint tlookup {A : Type} (f : string) l : option A := match l with
+    | [] => None
+    | (f', ty)::l' => if bool_decide (f = f') then Some ty else tlookup f l'
+  end.
+
+  Lemma type_rcons_instr E L l p1 p2 t1 t2: 
     ⊢ typed_instruction_ty E L [p1 ◁ t1 ; p2 ◁ t2] (l r: p1 :r: p2) (rcons (l, t1) t2).
   Proof.
     iIntros (tid ?) "_ _ $ $ (Hp1 & Hp2 & _)".
@@ -132,4 +163,86 @@ Context `{!typeGS Σ}.
     rewrite tctx_interp_singleton tctx_hasty_val.
     simpl. eauto with iFrame.
   Qed.
+
+  Fixpoint flatten v := match v with
+    | (f r: v1 :r: v2)%V => (f, v1) :: flatten v2
+    | _ => []
+  end.
+  Inductive record_val : val → Prop :=
+    | RVNil : record_val rnil%V
+    | RVCons f v' v1 : record_val v1 → record_val (f r: v' :r: v1).
+  Lemma flatten_eq v f : lang.tlookup v f = tlookup f (flatten v).
+  Proof.
+    induction v; try done.
+    simpl.
+    case_bool_decide; done.
+  Qed.
+
+  Lemma ty_own_lookup_val fs v f tid ty :
+    tlookup f fs = Some ty →
+    ty_own (record fs) tid [v] -∗
+    ∃v', ⌜lang.tlookup v f = Some v'⌝.
+  Proof.
+    iIntros (?) "Hown".
+    rewrite flatten_eq.
+    destruct fs as [| (?, ?) ?]; try done.
+    replace (record ((s, t) :: fs)) with (rcons (s, t) (record fs)) by done.
+    rewrite /rcons /=; iDestruct "Hown" as (??) "[% _]".
+    iPureIntro. simpl.
+    (* destruct v; try done. *)
+    revert v1 v2  H0.
+    induction v as [ | | | ]; try done.
+    simpl.
+    intros. simpl in H0.
+    assert (l = s) by admit.
+    assert (v0 = v1) by admit.
+    assert (v2 = v3) by admit.
+    subst.
+    case_bool_decide.
+    - by exists v1.
+    - admit.
+    (* FIXME: I belive the proof method is wrong, 
+    I might need to generalize something somewhere, also, I think I'll need to associate the return value and the type *)
+  Admitted.
+
+  Lemma type_proj_instr E L f p fs ty :
+    tlookup f fs = Some ty →
+    ⊢ typed_instruction_ty E L [p ◁ record fs] (p ↓ f) ty.
+  Proof.
+    iIntros (Hlookup tid ?) "_ _ $ $ Hp".
+    rewrite tctx_interp_singleton.
+    wp_apply (wp_hasty with "Hp").
+    iIntros (v) "_ Hown".
+    iDestruct (ty_own_lookup_val with "Hown") as "%H"; first apply Hlookup.
+    destruct H.
+    iApply wp_proj; first apply H. (* I need to get the value from record *)
+    admit.
+  Admitted.
+
+  Lemma type_rcons' E L C T T' p ty x e f:
+    Closed (x :b: []) e →
+    tctx_extract_ctx E L [p ◁ ty] T T' →
+    (∀ (v : val), typed_body E L C ((v ◁ rcons (f, ty) rnil') :: T') (subst' x v e)) -∗
+    typed_body E L C T (let: x := (f r: p :r: rnil) in e).
+  Proof. iIntros. iApply type_let; [iApply type_rcons_instr| |done]. 
+    admit.
+  Admitted.
+
+  Lemma type_rcons E L C T T' p1 p2 ty1 ty2 x e f:
+    Closed (x :b: []) e →
+    tctx_extract_ctx E L [p1 ◁ ty1; p2 ◁ ty2] T T' →
+    (∀ (v : val), typed_body E L C ((v ◁ rcons (f, ty1) ty2) :: T') (subst' x v e)) -∗
+    typed_body E L C T (let: x := (f r: p1 :r: p2) in e).
+  Proof. iIntros. iApply type_let; [iApply type_rcons_instr|solve_typing|done]. Qed.
+
+  Lemma type_proj E L C T T' p ty x e f fs:
+    Closed (x :b: []) e →
+    tlookup f fs = Some ty →
+    tctx_extract_ctx E L [p ◁ record fs] T T' →
+    (∀ (v : val), typed_body E L C ((v ◁ ty) :: T') (subst' x v e)) -∗
+    typed_body E L C T (let: x := p ↓ f in e).
+  Proof. iIntros. iApply type_let; [by iApply type_proj_instr|solve_typing|done]. Qed.
+
 End typing.
+Global Arguments record : simpl never.
+Global Arguments rcons : simpl never.
