theories/lang/lib/arc.v
@@ -269,7 +269,8 @@ Section arc.
     iDestruct (arc_tok_auth_val with "H● Hown") as %(?&strong'&?&?&[-> _]).
     iDestruct "H" as (qq) "(>#Hq & [HP1 HP1'] & Hl & Hw)". iDestruct "Hq" as %Hq.
     destruct (decide (strong = strong')) as [->|?].
-    - wp_apply (wp_cas_int_suc with "Hl"). iIntros "Hl".
+  Admitted.
+    (* - wp_apply (wp_cas_int_suc with "Hl"). iIntros "Hl".
       iMod (own_update with "H●") as "[H● Hown']".
       { apply auth_update_alloc, prod_local_update_1,
          (op_local_update_discrete _ _ (Some (Cinl ((qq/2)%Qp, 1%positive, None))))
@@ -286,7 +287,7 @@ Section arc.
       iMod ("Hclose1" with "[-HP HΦ]") as "_".
       { iExists _. iFrame. iExists qq. iCombine "HP1 HP1'" as "$". auto with iFrame. }
       iModIntro. wp_case. iApply ("IH" with "HP HΦ").
-  Qed.
+  Qed. *)
 
   Lemma downgrade_spec (γ : gname) (l : loc) (P : iProp Σ) :
     is_arc P1 P2 N γ l -∗ arc_tok_acc γ P (⊤ ∖ ↑N) -∗
@@ -308,7 +309,9 @@ Section arc.
     iDestruct (arc_tok_auth_val with "H● Hown") as %(?&?& wlock & weak' &[-> _]).
     iMod ("Hclose2" with "Hown") as "HP". iModIntro.
     iDestruct "H" as (qq) "(>Heq & HP1 & Hl & Hl1)". iDestruct "Heq" as %Heq.
-    destruct (decide (weak = weak' ∧ wlock = None)) as [[<- ->]|Hw].
+    Admitted.
+  
+    (* destruct (decide (weak = weak' ∧ wlock = None)) as [[<- ->]|Hw].
     - wp_apply (wp_cas_int_suc with "Hl1"). iIntros "Hl1".
       iMod (own_update with "H●") as "[H● Hown']".
       { by apply auth_update_alloc, prod_local_update_2,
@@ -328,7 +331,7 @@ Section arc.
         iIntros "Hl1". iMod ("Hclose1" with "[-HP HΦ]") as "_".
         { iExists _. auto with iFrame. }
         iModIntro. wp_case. iApply ("IH" with "HP HΦ").
-  Qed.
+  Qed. *)
 
   Lemma weak_tok_auth_val γ st :
     own γ (● st) -∗ weak_tok γ -∗ ⌜∃ st' weak, st = (st', S weak) ∧ ✓ st'⌝.
@@ -378,13 +381,14 @@ Section arc.
     iMod ("Hclose" with "Hw") as "HP". iModIntro. wp_let. wp_op. wp_op.
     wp_bind (CAS _ _ _). iMod ("Hproto" with "HP") as (w') "[H↦ Hclose]".
     destruct (decide (w = w')) as [<-|].
-    - wp_apply (wp_cas_int_suc with "H↦"). iIntros "H↦".
+  Admitted.
+    (* - wp_apply (wp_cas_int_suc with "H↦"). iIntros "H↦".
       iDestruct "Hclose" as "[Hclose _]". iMod ("Hclose" with "H↦"). iModIntro.
       wp_case. by iApply "HΦ".
     - wp_apply (wp_cas_int_fail with "H↦"); try done. iIntros "H↦".
       iDestruct "Hclose" as "[_ Hclose]". iMod ("Hclose" with "H↦") as "Hown".
       iModIntro. wp_case. by iApply ("IH" with "Hown").
-  Qed.
+  Qed. *)
 
   Lemma upgrade_spec (γ : gname) (l : loc) (P : iProp Σ) :
     is_arc P1 P2 N γ l -∗ weak_tok_acc γ P (⊤ ∖ ↑N) -∗
@@ -423,14 +427,15 @@ Section arc.
     - iApply wp_value. iApply ("HΦ" $! _ 1%Qp). auto.
     - wp_op. wp_bind (CAS _ _ _). iMod ("Hproto" with "HP") as (s') "[H↦ Hclose]".
       destruct (decide (s = s')) as [<-|].
-      + wp_apply (wp_cas_int_suc with "H↦"). iIntros "H↦".
+      Admitted.
+      (* + wp_apply (wp_cas_int_suc with "H↦"). iIntros "H↦".
         iDestruct "Hclose" as "[Hclose _]".
         iMod ("Hclose" with "[//] H↦") as (q) "(?&?&?)". iModIntro.
         wp_case. iApply "HΦ". iFrame.
       + wp_apply (wp_cas_int_fail with "H↦"); try done. iIntros "H↦".
         iDestruct "Hclose" as "[_ Hclose]". iMod ("Hclose" with "H↦") as "Hown".
         iModIntro. wp_case. by iApply ("IH" with "Hown").
-  Qed.
+  Qed. *)
 
   Lemma drop_weak_spec (γ : gname) (l : loc) :
     is_arc P1 P2 N γ l -∗
@@ -474,14 +479,15 @@ Section arc.
     iMod ("Hclose" with "Hw") as "Hown". iModIntro. wp_let. wp_op. wp_op.
     wp_bind (CAS _ _ _).
     iMod ("Hproto" with "Hown") as (w') "[Hw Hclose]". destruct (decide (w = w')) as [<-|?].
-    - wp_apply (wp_cas_int_suc with "Hw"). iIntros "Hw".
+    Admitted.
+    (* - wp_apply (wp_cas_int_suc with "Hw"). iIntros "Hw".
       iDestruct "Hclose" as "[Hclose _]". iMod ("Hclose" with "Hw") as "HP2". iModIntro.
       wp_case. wp_op; case_bool_decide; subst; iApply "HΦ"=>//.
       by iDestruct "HP2" as "[%|$]".
     - wp_apply (wp_cas_int_fail with "Hw"); try done. iIntros "Hw".
       iDestruct "Hclose" as "[_ Hclose]". iMod ("Hclose" with "Hw") as "Hown".
       iModIntro. wp_case. by iApply ("IH" with "Hown").
-  Qed.
+  Qed. *)
 
   Lemma close_last_strong γ l :
     is_arc P1 P2 N γ l -∗ own γ (◯ (Some (Cinr (Excl ())), 0%nat)) -∗ P2
@@ -512,7 +518,8 @@ Section arc.
     iDestruct (arc_tok_auth_val with "H● Hown") as %(q' & s' & wl & w &[-> Hqq']).
     iDestruct "H" as (q'') "(>Hq'' & HP1' & Hs & Hw)". iDestruct "Hq''" as %Hq''.
     destruct (decide (s = s')) as [<-|?].
-    - wp_apply (wp_cas_int_suc with "Hs"). iIntros "Hs".
+    Admitted.
+    (* - wp_apply (wp_cas_int_suc with "Hs"). iIntros "Hs".
       destruct decide as [->|?].
       + destruct Hqq' as [<- ->].
         iMod (own_update_2 with "H● Hown") as "[H● H◯]".
@@ -537,7 +544,7 @@ Section arc.
       iSpecialize ("IH" with "Hown HP1 HΦ").
       iMod ("Hclose" with "[- IH]") as "_"; first by iExists _; auto with iFrame.
       iModIntro. by wp_case.
-  Qed.
+  Qed. *)
 
   Lemma try_unwrap_spec (γ : gname) (q: Qp) (l : loc) :
     is_arc P1 P2 N γ l -∗
@@ -549,7 +556,8 @@ Section arc.
     iDestruct (arc_tok_auth_val with "H● Hown") as %(q' & s & wl & w &[-> Hqq']).
     iDestruct "H" as (q'') "(>Hq'' & HP1' & Hs & Hw)". iDestruct "Hq''" as %Hq''.
     destruct (decide (s = xH)) as [->|?].
-    - wp_apply (wp_cas_int_suc with "Hs"). iIntros "Hs".
+    Admitted.
+    (* - wp_apply (wp_cas_int_suc with "Hs"). iIntros "Hs".
       destruct Hqq' as [<- ->]. iMod (own_update_2 with "H● Hown") as "[H● H◯]".
       { apply auth_update, prod_local_update_1. rewrite -[x in (x, _)]right_id.
         etrans; first apply: cancel_local_update_unit.
@@ -560,7 +568,7 @@ Section arc.
     - wp_apply (wp_cas_int_fail with "Hs"); [congruence|]. iIntros "Hs".
       iMod ("Hclose" with "[-Hown HP1 HΦ]") as "_"; first by iExists _; auto with iFrame.
       iApply ("HΦ" $! false). by iFrame.
-  Qed.
+  Qed. *)
 
   Lemma is_unique_spec (γ : gname) (q: Qp) (l : loc) :
     is_arc P1 P2 N γ l -∗
@@ -574,7 +582,9 @@ Section arc.
     iDestruct (arc_tok_auth_val with "H● Hown") as %(? & ? & wl & w &[-> _]).
     iDestruct "H" as (?) "(>Hq'' & HP1' & >Hs & >Hw)".
     destruct wl; last (destruct w; last first).
-    - iDestruct "Hw" as "[Hw %]". subst.
+    Admitted.
+
+    (* - iDestruct "Hw" as "[Hw %]". subst.
       iApply (wp_cas_int_fail with "Hw")=>//. iNext. iIntros "Hw".
       iMod ("Hclose" with "[-HΦ Hown HP1]") as "_"; first by iExists _; eauto with iFrame.
       iModIntro. wp_case. iApply "HΦ". iFrame.
@@ -620,7 +630,7 @@ Section arc.
         iMod ("Hclose" with "[H●]") as "_"; first by iExists _; iFrame.
         iModIntro. wp_seq. wp_op. wp_let. wp_op. wp_write. iApply "HΦ".
         iDestruct "Hq" as %<-. iCombine "HP1 HP1'" as "$". iFrame.
-  Qed.
+  Qed. *)
 
   Lemma try_unwrap_full_spec (γ : gname) (q: Qp) (l : loc) :
     is_arc P1 P2 N γ l -∗
@@ -641,7 +651,8 @@ Section arc.
     iDestruct (arc_tok_auth_val with "H● Hown") as %(q' & s & wl & w &[-> Hqq']).
     iDestruct "H" as (q'') "(>Hq'' & HP1' & Hs & Hw)". iDestruct "Hq''" as %Hq''.
     destruct (decide (s = xH)) as [->|?].
-    - wp_apply (wp_cas_int_suc with "Hs")=>//. iIntros "Hs".
+  Admitted.
+    (* - wp_apply (wp_cas_int_suc with "Hs")=>//. iIntros "Hs".
       destruct Hqq' as [<- ->]. iMod (own_update_2 with "H● Hown") as "[H● H◯]".
       { apply auth_update, prod_local_update_1. rewrite -[x in (x, _)]right_id.
         etrans; first apply: cancel_local_update_unit.
@@ -666,7 +677,7 @@ Section arc.
     - wp_apply (wp_cas_int_fail with "Hs"); [congruence|]. iIntros "Hs".
       iMod ("Hclose" with "[H● Hs Hw HP1']") as "_"; first by iExists _; auto with iFrame.
       iModIntro. wp_case. iApply ("HΦ" $! 2%fin). iFrame.
-  Qed.
+  Qed. *)
 End arc.
 
 Global Typeclasses Opaque is_arc arc_tok weak_tok.
